Update

VRF/Spec.VRF.fst
@@ -3,31 +3,67 @@ module Spec.VRF
 open FStar.UInt32
 open FStar.UInt8
 open FStar.Seq
+open FStar.Option
 
-
-let prime = pow2 255 - 19
-let n = 2
-type elem: Type0 = e: int{e>=0 /\ e < prime}
-type point = | Proj: x: elem -> y: elem -> point
-
-
+open FStar.Mul
+open FStar.Seq
+open FStar.UInt8
+open FStar.Endianness
+open Spec.Lib
+open Spec.Curve25519.Lemmas
+open Spec.Curve25519
 
 let bytes =  seq FStar.UInt8.t
-let lbytes (l: nat) = b: seq UInt8.t {length b = l}
 let key = lbytes 32
-
 let order = 2
+let field = 100000000000
 
-assume val scalarAddition: p: point -> q: point -> Tot(r: point)
-assume val scalarMultiplication : p: point -> k: key -> Tot(r: point)
+let positive_point_const = Seq.create 1 2uy
+let negative_point_const = Seq.create 1 3uy
 
-assume val haclScalarMultiplication : p: point -> k: key -> Tot(point)
+assume val scalarMultiplication: point:serialized_point -> k: scalar -> Tot serialized_point
+assume val scalarAddition: p: serialized_point -> q: serialized_point -> Tot serialized_point
+assume val isPointOnCurve: p: option serialized_point -> Tot(bool)
 
-(*let op_Star_At = scalarAddition  *)
-let op_Star_Star = scalarMultiplication
+assume val _ECP2OS : gamma: serialized_point -> Tot(bytes)
+assume val _OS2ECP : bytes -> Tot(serialized_point)
+assume val _I2OSP: value1: int -> n: int -> Tot(bytes)
+assume val _OS2IP: bytes -> nat
 
-assume val _ECVRF_hash_to_curve: input: bytes -> 
-            public_key: 'a -> Tot(point)
+assume val hash: a: bytes -> Tot(bytes)
+
+val seqConcat : s1: seq 'a -> s2: seq 'a -> 
+            Tot(r:seq 'a{Seq.length    r = Seq.length s1 + Seq.length s2})
+
+let seqConcat s1 s2 = 
+    FStar.Seq.append s1 s2             
+
+val _helper_ECVRF_hash_to_curve : 
+    ctr : nat -> input: bytes -> pk: bytes -> Tot(r: option serialized_point{isPointOnCurve r})(decreases(field - ctr))
+
+let rec _helper_ECVRF_hash_to_curve ctr input pk = 
+    let _CTR = _I2OSP ctr 4 in 
+    let toHash = seqConcat input pk in 
+    let toHash = seqConcat toHash _CTR in 
+    let hash = hash toHash in 
+    let possible_point = seqConcat positive_point_const hash in 
+        if isPointOnCurve (Some possible_point) then Some possible_point 
+        else
+            let possible_point    = seqConcat negative_point_const hash in 
+                if isPointOnCurve (Some possible_point) then Some possible_point 
+                else 
+                    if (ctr +1) < field 
+                        then _helper_ECVRF_hash_to_curve (ctr+1) input pk 
+                    else None    
+
+
+val _ECVRF_hash_to_curve: input: bytes -> 
+            public_key: (serialized_point) -> Tot(option serialized_point)            
+
+let _ECVRF_hash_to_curve input public_key = 
+    let ctr = 0 in 
+    let pk = _ECP2OS public_key in 
+    let point = _helper_ECVRF_hash_to_curve ctr input pk in point
 
 assume val random:     max: nat{max < pow2 256} -> Tot(random : nat {random <= max})    
 assume val natToBytes : number : nat {number < pow2 256} -> Tot(key)    
@@ -36,38 +72,46 @@ val randBytes: max: nat{max < pow2 256} -> Tot(key)
 let randBytes max = 
     let rand = random max in natToBytes rand
 
-assume val _ECVRF_hash_points : generator: point -> h:  point -> 
-            public_key: point -> gamma : point -> 
-            gk : point -> hk : point -> 
+val _ECVRF_hash_points : generator: serialized_point -> h:  serialized_point -> 
+            public_key: serialized_point -> gamma : serialized_point -> 
+            gk : serialized_point -> hk : serialized_point -> 
             Tot(int)
 
-assume val pointToBytesTemp: a: point -> Tot(key)
+let _ECVRF_hash_points generator h public_key gamma gk hk = 
+    let p = _ECP2OS generator in 
+    let p = seqConcat p (_ECP2OS h) in 
+    let p = seqConcat p (_ECP2OS public_key) in 
+    let p = seqConcat p (_ECP2OS gamma) in 
+    let p = seqConcat p (_ECP2OS gk) in 
+    let p = seqConcat p (_ECP2OS hk) in 
+    let h' = hash p in 
+    let h = fst (FStar.Seq.split h' n) in 
+    _OS2IP h
 
-assume val _ECP2OS : gamma: point -> Tot(bytes)
-assume val _I2OSP: value1: int -> n: int -> Tot(bytes)
+assume val pointToBytesTemp: a: serialized_point -> Tot(key)
 
-assume val seqConcat : s1: seq 'a -> s2: seq 'a -> 
-            Tot(r:seq 'a{Seq.length    r = Seq.length s1 + Seq.length s2})
-
-val _ECVRF_prove: input: bytes ->  public_key: point -> 
-            private_key : point -> generator : point-> Tot(bytes) 
+val _ECVRF_prove: input: bytes ->  public_key: serialized_point -> 
+            private_key : serialized_point -> generator : serialized_point-> Tot(option bytes) 
             (*) Tot(proof: bytes{Seq.len proof = 5 * n + 1}) *)
 
 let _ECVRF_prove input public_key private_key generator = 
     let h = _ECVRF_hash_to_curve input public_key in 
-    let private_key_as_bytes = pointToBytesTemp private_key in 
-    let gamma = scalarMultiplication h private_key_as_bytes in 
-    let k_ = random (order-1) in 
-    let k =  natToBytes k_ in  
-    let gk = scalarMultiplication generator k in  (* k< (2^8)^32 = 2^(8*32) = 2^(2^3 * 2^ 5 = 256) *) (* *)
-    let hk = scalarMultiplication h k in 
-    let c = _ECVRF_hash_points generator h public_key gamma gk hk in (*int*)
-    let cq = op_Multiply c  prime in  (*int*)
-    let s = k_ - cq (* int *) in 
-    let fst = _ECP2OS gamma in 
-    let snd = _I2OSP c n in 
-    let thd = _I2OSP s ( op_Multiply 2 n) in 
-    let pi = seqConcat fst (seqConcat snd thd) in pi
+        if isNone h then None 
+        else 
+            let h = get h in     
+            let private_key_as_bytes = pointToBytesTemp private_key in 
+            let gamma = scalarMultiplication h private_key_as_bytes in 
+            let k_ = random (order-1) in 
+            let k =  natToBytes k_ in  
+            let gk = scalarMultiplication generator k in  (* k< (2^8)^32 = 2^(8*32) = 2^(2^3 * 2^ 5 = 256) *) (* *)
+            let hk = scalarMultiplication h k in 
+            let c = _ECVRF_hash_points generator h public_key gamma gk hk in (*int*)
+            let cq = op_Multiply c  prime in  (*int*)
+            let s = k_ - cq (* int *) in 
+            let fst = _ECP2OS gamma in 
+            let snd = _I2OSP c n in 
+            let thd = _I2OSP s ( op_Multiply 2 n) in 
+            let pi = seqConcat fst (seqConcat snd thd) in Some pi
 
 
 val _ECVRF_rec : counter: nat -> counter_local: nat{counter_local < counter} -> 
@@ -88,27 +132,29 @@ let _ECVRF_proof2hash pi =
 
 
 assume val _ECVRF_decode_proof: 
-        pi: bytes {Seq.length pi = op_Multiply 5 n + 1} -> Tot(point * key * key)
+        pi: bytes {Seq.length pi = op_Multiply 5 n + 1} -> 
+        Tot(tuple3 (option serialized_point) key key)
 
 
-val _ECVRF_verify : generator: point ->  public_key : point ->
+val _ECVRF_verify : generator: serialized_point ->  public_key : serialized_point ->
         pi: bytes {Seq.length pi = op_Multiply 5 n +1} -> 
         input : bytes -> 
         Tot(bool)
-
-assume val _isPointOnTheCurve :  p: point -> Tot(bool)        
-
-assume val equal : s1: bytes -> s2: bytes -> Tot(bool)
 
 assume val bytesToInt: s: bytes -> Tot(int)
 
 let _ECVRF_verify generator public_key pi input = 
     let gamma, c, s = _ECVRF_decode_proof pi in 
-    if not(_isPointOnTheCurve gamma) then false else
+    if not(isPointOnCurve gamma) then false else
+    if isNone gamma then false
+        else let gamma = get gamma in 
     let pkc = scalarMultiplication public_key c in 
     let gs = scalarMultiplication generator s in 
     let u  = scalarAddition pkc gs in 
     let h = _ECVRF_hash_to_curve input public_key in 
+        if isNone h then false
+    else 
+    let h = get h in 
     let gammac = scalarMultiplication gamma c in 
     let hs = scalarMultiplication h s in 
     let v = scalarAddition gammac hs in 
